src/lowparse/LowParse.Spec.List.fst
@@ -65,6 +65,7 @@ let parse_list_bare_consumes_all
   (consumes_all (parse_list_bare p))
 = Classical.forall_intro (Classical.move_requires (parse_list_bare_consumed p))
 
+(*
 let no_lookahead_weak_on_parse_list_bare
   (#t: Type0)
   (p: bare_parser t)
@@ -74,6 +75,7 @@ let no_lookahead_weak_on_parse_list_bare
 = match parse_list_bare p x with
   | Some _ -> parse_list_bare_consumed p x
   | _ -> ()
+*)
 
 #set-options "--z3rlimit 16"
 
@@ -136,7 +138,7 @@ val parse_list
 : Tot (parser parse_list_kind (list t))
 
 let parse_list #k #t p =
-  Classical.forall_intro_2 (no_lookahead_weak_on_parse_list_bare p);
+//  Classical.forall_intro_2 (no_lookahead_weak_on_parse_list_bare p);
   parse_list_bare_injective p;
   parse_list_bare_consumes_all p;
   parse_list_bare p
